TM/Basic/Nop.v
@@ -13,7 +13,7 @@ Section Nop.
     induction tapes; cbn in *; eauto using f_equal.
   Qed.
 
-  Definition nop_trans := fun (p : (FinType (EqType unit)) * Vector.t (option sig) (S n))  => let (q,a) := p in (q, null_action (S n)).
+  Definition nop_trans := fun (p : (FinType (EqType unit)) * Vector.t (option sig) n)  => let (q,a) := p in (q, null_action n).
 
   Definition nop : mTM sig n :=
     Build_mTM nop_trans tt (fun _ => true).
