TM/Combinators/If.v
@@ -34,8 +34,8 @@ Section Composition.
     projT1 pM1 ↓ T1 ->
     projT1 pM2 ↓ T2 ->
     projT1 pM3 ↓ T3 ->
-    projT1 If ↓ (fun (t : tapes sig (S n)) (i : nat) =>
-            exists (i1 i2 : nat) (b : bool) (y : tapes sig (S n)),
+    projT1 If ↓ (fun (t : tapes sig n) (i : nat) =>
+            exists (i1 i2 : nat) (b : bool) (y : tapes sig n),
               i > i1 + i2 /\
               (R1 t (b, y) /\ b = true /\ T1 t i1 /\ T2 y i2 \/
                                                   R1 t (b, y) /\ b = false /\ T1 t i1 /\ T3 y i2)).
